\subsection{Prove that $\sum_{i=1}^{n} i = n(n+1)/2$ for $n \geq 0$, by induction}
  \textbf{Question number:} 1-10.

  \begin{proof}[Proof by induction]

    For any integer value $n > 0$, let $P(n)$ denote the statement $P(n) = (\sum_{i=1}^n i \doteq n(n+1)/2)$.

    \textbf{Base step $(n=1)$}

    \begin{align}
      P(1) &= 1(1+1)/2\\
           &= 1(2)/2\\
           &= 2/2\\
           &= 1
    \end{align}

    Thus, the base step is true.

    \textbf{Inductive step}
    Assume all of $P(1), ..., P(n)$ are true. Then we show that $P(n+1)$ is true as well:

    Calculating the value of $P(n+1)$ for left hand side
    \begin{align}
      P(n+1) &= P(n) + (n + 1)\\
             &= (n(n+1)/2) + (n+1)\\
             &= (n^2+n/2) + (n+1)\\
             &= ((n^2+n) + 2(n+1))/2\\
             &= (n^2+n + 2n+2)/2\\
             &= (n^2+3n+2)/2\\
    \end{align}

    Calculating the value of $\sum_{i=1}^n i$ for right hand side
    \begin{align}
      \sum_{i=1}^n i &= ((n+1)((n+1)+1))/2\\
                     &= (n+1)(n+2)/2\\
                     &= (n^2+2n+n+2)/2\\
                     &= (n^2+3n+2)/2\\
    \end{align}

    Both left hand side and right hand side is equal, thus it proves that the
    equation $n(n+1)/2$ to find the sum of all the integers from $1$ to $n$ is
    true.
    \qedhere
  \end{proof}
